execute the tasks

dafny/example/json_model.dfy
@@ -1,8 +1,8 @@
 /**
   * Direct JSON to ProcessDefinition conversion
   */
-include "process.dfy"
-include "utils/option.dfy"
+include "../src/process.dfy"
+include "../src/utils/option.dfy"
 
 module JsonModel {
   import opened ProcessDefinition
@@ -12,16 +12,25 @@ module JsonModel {
     * Python script generates this function directly
     */
   function CreateParsedModel01(): ProcessDef
+    ensures |CreateParsedModel01().startNodes| == 1
+    ensures |CreateParsedModel01().endNodes| > 0
+    ensures forall startNodeId :: startNodeId in CreateParsedModel01().startNodes ==>
+                                    startNodeId in CreateParsedModel01().nodes
+    ensures forall endNodeId :: endNodeId in CreateParsedModel01().endNodes ==>
+                                  endNodeId in CreateParsedModel01().nodes
+    ensures forall startNodeId :: startNodeId in CreateParsedModel01().startNodes ==>
+                                    CreateParsedModel01().nodes[startNodeId].incoming == {}
+
   {
     var nodes := map[
-                   "StartEvent_1" := ProcessNode("StartEvent_1", "Start", StartEvent, {}, {"t0"}),
+                   "StartEvent_1" := ProcessNode("StartEvent_1", "Start", StartEvent, {}, {"flow_start_t0"}),
                    "EndEvent_16dmtu6" := ProcessNode("EndEvent_16dmtu6", "End", EndEvent, {"ExclusiveGateway_0ms7zfc"}, {}),
-                   "t0" := ProcessNode("t0", "Which option?", Task(UserTask), {"StartEvent_1"}, {"ParallelGateway_05lp38c"}),
-                   "tup" := ProcessNode("tup", "Up", Task(UserTask), {"ParallelGateway_05lp38c"}, {"ParallelGateway_0vffee4"}),
-                   "tdown" := ProcessNode("tdown", "Down", Task(UserTask), {"ParallelGateway_05lp38c"}, {"ParallelGateway_0vffee4"}),
-                   "ParallelGateway_05lp38c" := ProcessNode("ParallelGateway_05lp38c", "Split", Gateway(ParallelGateway), {"t0"}, {"tup", "tdown"}),
-                   "ParallelGateway_0vffee4" := ProcessNode("ParallelGateway_0vffee4", "Join", Gateway(ParallelGateway), {"tup", "tdown"}, {"mt"}),
-                   "ExclusiveGateway_0ms7zfc" := ProcessNode("ExclusiveGateway_0ms7zfc", "Merge", Gateway(ExclusiveGateway), {"tup2", "tdown2"}, {"EndEvent_16dmtu6"})
+                   "t0" := ProcessNode("t0", "Which option?", Task(UserTask), {"flow_start_t0"}, {"flow_t0_split"}),
+                   "tup" := ProcessNode("tup", "Up", Task(UserTask), {"flow_t0_split"}, {"flow_split_up"}),
+                   "tdown" := ProcessNode("tdown", "Down", Task(UserTask), {"flow_t0_split"}, {"flow_split_down"}),
+                   "ParallelGateway_05lp38c" := ProcessNode("ParallelGateway_05lp38c", "Split", Gateway(ParallelGateway), {"flow_t0_split"}, {"flow_split_up", "flow_split_down"}),
+                   "ParallelGateway_0vffee4" := ProcessNode("ParallelGateway_0vffee4", "Join", Gateway(ParallelGateway), {"flow_split_up", "flow_split_down"}, {"flow_up_join", "flow_down_join"}),
+                   "ExclusiveGateway_0ms7zfc" := ProcessNode("ExclusiveGateway_0ms7zfc", "Merge", Gateway(ExclusiveGateway), {"flow_up_join", "flow_down_join"}, {"flow_join_end"})
                  ];
 
     var flows := map[
