dafny/src/engine.dfy
@@ -1,4 +1,4 @@
-/**
+/** 
   * Core Execution Engine
   */
 
@@ -6,35 +6,78 @@ include "./token.dfy"
 include "./state.dfy"
 include "./process.dfy"
 include "./utils/variables.dfy"
+include "./execution_init.dfy"
 module ExecutionEngine {
   import opened Token
   import opened BPMNState
   import opened ProcessDefinition
   import opened Variables
+  import opened ExecutionInit
 
   /**
     * The main execution function
     */
-  function ExecuteStep(state: State): State
-    requires state.Running?
+  function ExecuteStep(state: ExecutingState): State
     requires ValidState(state)
-    ensures ValidState(ExecuteStep(state))
   {
     var process := state.process;
     var activeTokens := GetActiveTokens(process.tokenCollection);
 
-    if |activeTokens| == 0 then
-      Completed(process, process.globalVariables)
-    else
-      var tokenId := Token.PickOne(activeTokens);
-      ExecuteTokenStep(state, tokenId)
+    // Since RunningProcess constraint, activeTokens is automatically non-empty
+    var tokenId := Token.PickOne(activeTokens);
+    var process := state.process;
+    var token := process.tokenCollection.tokens[tokenId];
+    var currentNode := process.processDefinition.nodes[token.location];
+    match currentNode.nodeType {
+      case StartEvent =>
+        if CanExecuteStartEvent(state) then
+          ExecuteStartEvent(state)
+        else
+          state  // or return error state
+      case EndEvent => ExecuteEndEvent(state, tokenId)
+      case Task(taskType) => ExecuteTask(state, tokenId, taskType)
+      case Gateway(gatewayType) => ExecuteGateway(state, tokenId, gatewayType)
+      case IntermediateEvent(eventType) => ExecuteIntermediateEvent(state, tokenId, eventType)
+    }
   }
 
+
+  // execute the step of a start event
+  function ExecuteStartEvent(state: State): State
+    requires CanExecuteStartEvent(state)
+    ensures ExecuteStartEvent(state).Running?
+  {
+    ExecutionInit.ProcessStartEvent(state)
+  }
+  // execute the step of a end event
+  function ExecuteEndEvent(state: State, tokenId: Token.TokenId): State { state }
+  // execute the step of a task
+  function ExecuteTask(state: ExecutingState, tokenId: Token.TokenId, taskType: TaskType): State
+    requires tokenId in GetActiveTokens(state.process.tokenCollection)
+    requires tokenId in state.process.tokenCollection.tokens
+    requires state.process.tokenCollection.tokens[tokenId].location in state.process.processDefinition.nodes
+  {
+    match taskType {
+      case UserTask =>
+        ExecuteUserTask(state, tokenId)
+      case ServiceTask =>
+        ExecuteServiceTask(state, tokenId)
+      case ManualTask =>
+        ExecuteManualTask(state, tokenId)
+    }
+  }
+  // execute the step of a gateway
+  function ExecuteGateway(state: ExecutingState, tokenId: Token.TokenId, gatewayType: GatewayType): State
+  {
+    state
+  }
+  // execute the step of a intermediate event
+  function ExecuteIntermediateEvent(state: State, tokenId: Token.TokenId, eventType: ProcessDefinition.EventType): State { state }
+
   /**
-    * Execute the step of a single token
+    * Execute a user task - for testing, we simulate user input
     */
-  function ExecuteTokenStep(state: State, tokenId: Token.TokenId): State
-    requires state.Running?
+  function ExecuteUserTask(state: ExecutingState, tokenId: Token.TokenId): State
     requires tokenId in GetActiveTokens(state.process.tokenCollection)
     requires tokenId in state.process.tokenCollection.tokens
     requires state.process.tokenCollection.tokens[tokenId].location in state.process.processDefinition.nodes
@@ -43,23 +86,129 @@ module ExecutionEngine {
     var token := process.tokenCollection.tokens[tokenId];
     var currentNode := process.processDefinition.nodes[token.location];
 
-    match currentNode.nodeType {
-      case StartEvent => ExecuteStartEvent(state, tokenId)
-      case EndEvent => ExecuteEndEvent(state, tokenId)
-      case Task(taskType) => ExecuteTask(state, tokenId, taskType)
-      case Gateway(gatewayType) => ExecuteGateway(state, tokenId, gatewayType)
-      case IntermediateEvent(eventType) => ExecuteIntermediateEvent(state, tokenId, eventType)
-    }
+    // Add process validation
+    var outgoingFlows := currentNode.outgoing;
+    if |outgoingFlows| == 1 then
+      var flowId := Token.PickOne(outgoingFlows);
+      if flowId in process.processDefinition.flows then
+        var nextNodeId := process.processDefinition.flows[flowId].targetRef;
+        // Simulate user completing task - consume current token, create next token
+        var tokensAfterConsume := Token.ConsumeToken(process.tokenCollection, tokenId);
+        var (tokensWithNext, nextTokenId) := Token.CreateToken(tokensAfterConsume, nextNodeId);
+
+        // Update execution history
+        var newHistory := process.executionHistory + [
+                            Event(0, token.location, NodeExited, tokenId, Variables.EmptyVariables()),
+                            Event(1, nextNodeId, NodeEntered, nextTokenId, Variables.EmptyVariables())
+                          ];
+
+        var updatedProcess := Process(
+                                processId := process.processId,
+                                tokenCollection := tokensWithNext,
+                                globalVariables := process.globalVariables,  // 可以在这里更新变量
+                                processDefinition := process.processDefinition,
+                                executionHistory := newHistory,
+                                context := process.context
+                              );
+
+        // Update context
+        var updatedContext := ExecutionContext.ComputeContext(
+                                updatedProcess.tokenCollection,
+                                nextNodeId,
+                                process.context
+                              );
+
+        Running(Process(
+                  processId := process.processId,
+                  tokenCollection := tokensWithNext,
+                  globalVariables := process.globalVariables,
+                  processDefinition := process.processDefinition,
+                  executionHistory := newHistory,
+                  context := updatedContext
+                ))
+      else
+        BPMNState.Error(process, ValidationError("Flow not found in process definition"))
+    else
+      // Multiple output flows - this is usually an error for UserTask
+      BPMNState.Error(process, ValidationError("UserTask should not have multiple outgoing flows"))
   }
 
-  // execute the step of a start event
-  function ExecuteStartEvent(state: State, tokenId: Token.TokenId): State { state }
-  // execute the step of a end event
-  function ExecuteEndEvent(state: State, tokenId: Token.TokenId): State { state }
-  // execute the step of a task
-  function ExecuteTask(state: State, tokenId: Token.TokenId, taskType: TaskType): State { state }
-  // execute the step of a gateway
-  function ExecuteGateway(state: State, tokenId: Token.TokenId, gatewayType: GatewayType): State { state }
-  // execute the step of a intermediate event
-  function ExecuteIntermediateEvent(state: State, tokenId: Token.TokenId, eventType: ProcessDefinition.EventType): State { state }
+  /**
+    * Execute a service task - automatic execution
+    */
+  function ExecuteServiceTask(state: ExecutingState, tokenId: Token.TokenId): State
+    requires tokenId in GetActiveTokens(state.process.tokenCollection)
+    requires tokenId in state.process.tokenCollection.tokens
+    requires state.process.tokenCollection.tokens[tokenId].location in state.process.processDefinition.nodes
+  {
+    ExecuteSimpleTask(state, tokenId, "ServiceTask")
+  }
+
+  /**
+    * Execute a manual task - requires human intervention
+    */
+  function ExecuteManualTask(state: ExecutingState, tokenId: Token.TokenId): State
+    requires tokenId in GetActiveTokens(state.process.tokenCollection)
+    requires tokenId in state.process.tokenCollection.tokens
+    requires state.process.tokenCollection.tokens[tokenId].location in state.process.processDefinition.nodes
+  {
+    ExecuteSimpleTask(state, tokenId, "ManualTask")
+  }
+
+  /**
+    * Common task execution logic
+    */
+  function ExecuteSimpleTask(state: ExecutingState, tokenId: Token.TokenId, taskType: string): State
+    requires tokenId in GetActiveTokens(state.process.tokenCollection)
+    requires tokenId in state.process.tokenCollection.tokens
+    requires state.process.tokenCollection.tokens[tokenId].location in state.process.processDefinition.nodes
+  {
+    var process := state.process;
+    var token := process.tokenCollection.tokens[tokenId];
+    var currentNode := process.processDefinition.nodes[token.location];
+
+    // 获取输出流
+    var outgoingFlows := currentNode.outgoing;
+    if |outgoingFlows| == 1 then
+      var flowId := Token.PickOne(outgoingFlows);
+      if flowId in process.processDefinition.flows then
+        var nextNodeId := process.processDefinition.flows[flowId].targetRef;
+        // 消费当前token
+        var tokensAfterConsume := Token.ConsumeToken(process.tokenCollection, tokenId);
+        var (tokensWithNext, nextTokenId) := Token.CreateToken(tokensAfterConsume, nextNodeId);
+
+        var newHistory := process.executionHistory + [
+                            Event(0, token.location, NodeExited, tokenId, Variables.EmptyVariables()),
+                            Event(1, nextNodeId, NodeEntered, nextTokenId, Variables.EmptyVariables())
+                          ];
+
+        var updatedProcess := Process(
+                                processId := process.processId,
+                                tokenCollection := tokensWithNext,
+                                globalVariables := process.globalVariables,
+                                processDefinition := process.processDefinition,
+                                executionHistory := newHistory,
+                                context := process.context
+                              );
+
+        // Update context
+        var updatedContext := ExecutionContext.ComputeContext(
+                                updatedProcess.tokenCollection,
+                                nextNodeId,
+                                process.context
+                              );
+
+        Running(Process(
+                  processId := process.processId,
+                  tokenCollection := tokensWithNext,
+                  globalVariables := process.globalVariables,
+                  processDefinition := process.processDefinition,
+                  executionHistory := newHistory,
+                  context := updatedContext
+                ))
+      else
+        BPMNState.Error(process, ValidationError("Flow not found in process definition"))
+    else
+      BPMNState.Error(process, ValidationError(taskType + " should have exactly one outgoing flow"))
+  }
 } 
