dafny/src/state.dfy
@@ -1,13 +1,18 @@
 /*
- *  Provide state type
+ * Provide state type
  */
 include "token.dfy"
 include "utils/variables.dfy"
 include "process.dfy"
+include "Context.dfy"
+include "utils/option.dfy"
+
 module BPMNState {
   import opened Token
   import opened Variables
   import opened ProcessDefinition
+  import opened ExecutionContext
+  import opened Optional
 
   /**
     * error code type
@@ -26,19 +31,19 @@ module BPMNState {
     tokenCollection: Token.Collection,
     globalVariables: Variables.VariableMap,
     processDefinition: ProcessDefinition.ProcessDef,
-    executionHistory: seq<ExecutionEvent>
+    executionHistory: seq<ExecutionEvent>,
+    context: ExecutionContext.Context
   )
 
   /**
-    * BPMN execution state
+    * BPMN execution state - reference EVM design
     */
   datatype State =
+    | NotStarted(processDefinition: ProcessDefinition.ProcessDef, initialVariables: Variables.VariableMap)
     | Running(process: ProcessObj)
     | Completed(process: ProcessObj, output: Variables.VariableMap)
     | Terminated(process: ProcessObj)
     | Error(process: ProcessObj, errorCode: ErrorCode)
-    | Compensating(process: ProcessObj)
-    | Waiting(process: ProcessObj, waitingFor: WaitCondition)
 
   /**
     * wait condition
@@ -76,8 +81,24 @@ module BPMNState {
     */
   predicate ValidState(state: State)
   {
-    state.Running? ==> Token.ValidTokenCollection(state.process.tokenCollection) &&
-                       ValidProcessState(state.process)
+    match state {
+      case NotStarted(processDefinition, initialVariables) =>
+        ValidProcessDefinition(processDefinition)
+      case Running(process) =>
+        Token.HasActiveTokens(process.tokenCollection) &&
+        Token.ValidTokenCollection(process.tokenCollection) &&
+        ValidProcessState(process)
+      case Completed(process, _) =>
+        !Token.HasActiveTokens(process.tokenCollection) &&
+        Token.ValidTokenCollection(process.tokenCollection) &&
+        ValidProcessState(process)
+      case Terminated(process) =>
+        Token.ValidTokenCollection(process.tokenCollection) &&
+        ValidProcessState(process)
+      case Error(process, _) =>
+        Token.ValidTokenCollection(process.tokenCollection) &&
+        ValidProcessState(process)
+    }
   }
 
   predicate ValidProcessState(process: ProcessObj)
@@ -86,5 +107,166 @@ module BPMNState {
     forall tokenId :: tokenId in GetActiveTokens(process.tokenCollection) ==>
                         tokenId in process.tokenCollection.tokens &&
                         process.tokenCollection.tokens[tokenId].location in process.processDefinition.nodes
+  }
+
+  /**
+    * validate process definition
+    */
+  predicate ValidProcessDefinition(processDefinition: ProcessDefinition.ProcessDef)
+  {
+    // at least one start node
+    |processDefinition.startNodes| > 0 &&
+    // at least one end node
+    |processDefinition.endNodes| > 0 &&
+    // start nodes are in the node collection
+    (forall nodeId :: nodeId in processDefinition.startNodes ==> nodeId in processDefinition.nodes) &&
+    // end nodes are in the node collection
+    (forall nodeId :: nodeId in processDefinition.endNodes ==> nodeId in processDefinition.nodes) &&
+    // all flow source and target nodes exist
+    (forall flowId :: flowId in processDefinition.flows ==>
+                        var flow := processDefinition.flows[flowId];
+                        flow.sourceRef in processDefinition.nodes && flow.targetRef in processDefinition.nodes)
+  }
+
+  /**
+    * create initial state
+    */
+  function CreateInitialState(processDefinition: ProcessDefinition.ProcessDef, initialVariables: Variables.VariableMap): State
+    requires ValidProcessDefinition(processDefinition)
+    ensures ValidState(CreateInitialState(processDefinition, initialVariables))
+  {
+    NotStarted(processDefinition, initialVariables)
+  }
+
+  /**
+    * check if process can complete
+    */
+  function CanComplete(state: State): bool
+    requires state.Running?
+  {
+    var process := state.process;
+    var activeTokens := Token.GetActiveTokens(process.tokenCollection);
+
+    // check if all active tokens are in end nodes
+    forall tokenId :: tokenId in activeTokens ==>
+                        process.tokenCollection.tokens[tokenId].location in process.processDefinition.endNodes
+  }
+
+  /**
+    * an executing state must have active tokens
+    | is subset type in Dafny
+    type TypeName = baseType | constraint
+    witness is used to create a simple example of the type, otherwise dafny complains about the type maybe empty
+    */
+  type ExecutingState = s:State | s.Running? && Token.HasActiveTokens(s.process.tokenCollection)
+    witness Running(BPMN_RUNNING_PROCESS_WITNESS)
+
+  /**
+    * a terminated state must not have active tokens
+    */
+  type TerminatedState = s:State | s.Terminated?
+    witness Terminated(BPMN_PROCESS_WITNESS)
+
+  /**
+    * a completed state must not have active tokens
+    */
+  type CompletedState = s:State | s.Completed? && !Token.HasActiveTokens(s.process.tokenCollection)
+    witness Completed(BPMN_PROCESS_WITNESS, Variables.EmptyVariables())
+
+  /**
+    * create a dummy process definition for witness
+    */
+  function CreateDummyProcessDef(): ProcessDef
+  {
+    ProcessDefinition(
+      id := "dummy",
+      name := "dummy",
+      nodes := map["start" := ProcessNode("start", "start", StartEvent, {}, {})],
+      flows := map[],
+      startNodes := {"start"},
+      endNodes := {}
+    )
+  }
+
+  const BPMN_PROCESS_WITNESS : ProcessObj := Process(
+                                               processId := "witness",
+                                               tokenCollection := Token.Create(),
+                                               globalVariables := Variables.EmptyVariables(),
+                                               processDefinition := CreateDummyProcessDef(),
+                                               executionHistory := [],
+                                               context := ExecutionContext.CreateInitialContext()
+                                             )
+
+  const BPMN_RUNNING_PROCESS_WITNESS : ProcessObj :=
+    var emptyTokens := Token.Create();
+    var (tokensWithOne, tokenId) := Token.CreateToken(emptyTokens, "dummy");
+    Process(
+      processId := "witness",
+      tokenCollection := tokensWithOne,
+      globalVariables := Variables.EmptyVariables(),
+      processDefinition := CreateDummyProcessDef(),
+      executionHistory := [],
+      context := ExecutionContext.CreateInitialContext()
+    )
+
+  /**
+    * State utility functions for location tracking
+    */
+
+  /**
+    * Get all current token locations
+    */
+  function GetCurrentLocations(state: State): set<string>
+    requires state.Running?
+  {
+    state.process.context.currentNodes
+  }
+
+  /**
+    * Get primary location (when single token)
+    */
+  function GetPrimaryLocation(state: State): Option<string>
+    requires state.Running?
+  {
+    var process := state.process;
+    var activeTokens := Token.GetActiveTokens(process.tokenCollection);
+    if |activeTokens| == 1 then
+      var tokenId := Token.PickOne(activeTokens);
+      Some(process.tokenCollection.tokens[tokenId].location)
+    else
+      None
+  }
+
+  /**
+    * Check if execution is at specific node
+    */
+  predicate IsAtNode(state: State, nodeId: string)
+    requires state.Running?
+  {
+    nodeId in state.process.context.currentNodes
+  }
+
+  /**
+    * Update ProcessObj's context
+    */
+  function UpdateProcessContext(
+    process: ProcessObj,
+    lastExecutedNode: string
+  ): ProcessObj
+  {
+    var updatedContext := ExecutionContext.ComputeContext(
+                            process.tokenCollection,
+                            lastExecutedNode,
+                            process.context
+                          );
+
+    Process(
+      processId := process.processId,
+      tokenCollection := process.tokenCollection,
+      globalVariables := process.globalVariables,
+      processDefinition := process.processDefinition,
+      executionHistory := process.executionHistory,
+      context := updatedContext
+    )
   }
 }
